Auto/Lib/BoolExtra.lean
@@ -30,4 +30,52 @@ theorem Bool.and_comm {a b : Bool} : (a && b) = (b && a) := by
 theorem Bool.or_comm {a b : Bool} : (a || b) = (b || a) := by
   cases a <;> cases b <;> decide
 
+noncomputable def Bool.ofProp (c : Prop) : Bool :=
+  match Classical.propDecidable c with
+  | .isTrue _ => true
+  | .isFalse _ => false
+
+theorem Bool.ofProp_spec (c : Prop) : Bool.ofProp c ↔ c := by
+  dsimp [ofProp]
+  cases h : Classical.propDecidable c <;> simp [*]
+
+theorem Bool.ofProp_spec' (c : Prop) : Bool.ofProp c = false ↔ ¬ c := by
+  conv => enter [2, 1]; rw [← Bool.ofProp_spec c]
+  simp
+
+/--
+  Similar to `Bool.cond`, but allows `Prop` argument
+-/
+def Bool.cond' {α : Sort u} (b : Bool) (x y : α) :=
+  match b with
+  | true => x
+  | false => y
+
+theorem Bool.ite_eq_true (p : Prop) [inst : Decidable p] (a b : α) : p → ite p a b = a := by
+  intro hp; dsimp [ite]; cases inst
+  case isFalse hnp => apply False.elim (hnp hp)
+  case isTrue _ => rfl
+
+theorem Bool.ite_eq_false (p : Prop) [inst : Decidable p] (a b : α) : ¬ p → ite p a b = b := by
+  intro hnp; dsimp [ite]; cases inst
+  case isFalse _ => rfl
+  case isTrue hp => apply False.elim (hnp hp)
+
+/--
+  Invoke `simp_only` at the beginning of `auto`
+-/
+theorem Bool.ite_simp {α : Sort u} (p : Prop) [Decidable p] (x y : α) :
+  ite p x y = cond' (Bool.ofProp p) x y := by
+  cases h : Bool.ofProp p
+  case false => rw [Bool.ite_eq_false]; rfl; apply (Bool.ofProp_spec' _).mp h
+  case true  => rw [Bool.ite_eq_true]; rfl; apply (Bool.ofProp_spec _).mp h
+
+/--
+  Invoke `simp_only` at the beginning of `auto`
+-/
+theorem Bool.decide_simp (p : Prop) [Decidable p] : decide p = Bool.ofProp p := by
+  cases h : Bool.ofProp p
+  case false => rw [decide_eq_false]; apply (Bool.ofProp_spec' _).mp h
+  case true  => rw [decide_eq_true]; apply (Bool.ofProp_spec _).mp h
+
 end Auto
