Test/SmtTranslation/BitVec.lean
@@ -27,6 +27,11 @@ example : (2 : BitVec 7).rotateRight 3 = (0x20 : BitVec 7) := by
 example (x : BitVec 15) : x.rotateLeft 3 = x.rotateRight 12 := by
   auto
 
+-- Issue: Permute!
+open BitVec in
+example : (2 : BitVec 7).rotateLeft 3 = 0b10000#7 := by
+  auto
+
 example :
   (2 : BitVec 7).rotateRight n = (2 : BitVec 7).rotateRight n ∧
   (3 : BitVec 7).rotateRight n = (3 : BitVec 7).rotateRight n ∧
